algebra/sts.v
@@ -5,120 +5,85 @@ Local Arguments valid _ _ !_ /.
 Local Arguments op _ _ !_ !_ /.
 Local Arguments unit _ _ !_ /.
 
+(** * Definition of STSs *)
 Module sts.
-
-Record stsT := STS {
+Structure stsT := STS {
   state : Type;
   token : Type;
-  trans : relation state;
-  tok   : state → set token;
+  prim_step : relation state;
+  tok : state → set token;
 }.
 Arguments STS {_ _} _ _.
+Arguments prim_step {_} _ _.
+Arguments tok {_} _.
+Notation states sts := (set (state sts)).
+Notation tokens sts := (set (token sts)).
 
-(* The type of bounds we can give to the state of an STS. This is the type
-   that we equip with an RA structure. *)
-Inductive bound (sts : stsT) :=
-  | bound_auth : state sts → set (token sts) → bound sts
-  | bound_frag : set (state sts) → set (token sts )→ bound sts.
-Arguments bound_auth {_} _ _.
-Arguments bound_frag {_} _ _.
+(** * Theory and definitions *)
+Section sts.
+Context {sts : stsT}.
 
-Section sts_core.
-Context (sts : stsT).
-Infix "≼" := dra_included.
-
-Notation state := (state sts).
-Notation token := (token sts).
-Notation trans := (trans sts).
-Notation tok := (tok sts).
-
-Inductive equiv : Equiv (bound sts) :=
-  | auth_equiv s T1 T2 : T1 ≡ T2 → bound_auth s T1 ≡ bound_auth s T2
-  | frag_equiv S1 S2 T1 T2 : T1 ≡ T2 → S1 ≡ S2 →
-                             bound_frag S1 T1 ≡ bound_frag S2 T2.
-Global Existing Instance equiv.
-Inductive step : relation (state * set token) :=
+(** ** Step relations *)
+Inductive step : relation (state sts * tokens sts) :=
   | Step s1 s2 T1 T2 :
-     trans s1 s2 → tok s1 ∩ T1 ≡ ∅ → tok s2 ∩ T2 ≡ ∅ →
+     prim_step s1 s2 → tok s1 ∩ T1 ≡ ∅ → tok s2 ∩ T2 ≡ ∅ →
      tok s1 ∪ T1 ≡ tok s2 ∪ T2 → step (s1,T1) (s2,T2).
-Hint Resolve Step.
-Inductive frame_step (T : set token) (s1 s2 : state) : Prop :=
+Inductive frame_step (T : tokens sts) (s1 s2 : state sts) : Prop :=
   | Frame_step T1 T2 :
      T1 ∩ (tok s1 ∪ T) ≡ ∅ → step (s1,T1) (s2,T2) → frame_step T s1 s2.
-Hint Resolve Frame_step.
-Record closed (S : set state) (T : set token) : Prop := Closed {
+
+(** ** Closure under frame steps *)
+Record closed (S : states sts) (T : tokens sts) : Prop := Closed {
   closed_ne : S ≢ ∅;
   closed_disjoint s : s ∈ S → tok s ∩ T ⊆ ∅;
   closed_step s1 s2 : s1 ∈ S → frame_step T s1 s2 → s2 ∈ S
 }.
-Lemma closed_disjoint' S T s :
-  closed S T → s ∈ S → tok s ∩ T ≡ ∅.
-Proof.
-  move=>Hcl Hin. move:(closed_disjoint _ _ Hcl _ Hin).
-  solve_elem_of+.
-Qed.
-Lemma closed_steps S T s1 s2 :
-  closed S T → s1 ∈ S → rtc (frame_step T) s1 s2 → s2 ∈ S.
-Proof. induction 3; eauto using closed_step. Qed.
-Global Instance valid : Valid (bound sts) := λ x,
-  match x with
-  | bound_auth s T => tok s ∩ T ≡ ∅ | bound_frag S' T => closed S' T
-  end.
-Definition up (s : state) (T : set token) : set state :=
+Definition up (s : state sts) (T : tokens sts) : states sts :=
   mkSet (rtc (frame_step T) s).
-Definition up_set (S : set state) (T : set token) : set state :=
+Definition up_set (S : states sts) (T : tokens sts) : states sts :=
   S ≫= λ s, up s T.
-Global Instance unit : Unit (bound sts) := λ x,
-  match x with
-  | bound_frag S' _ => bound_frag (up_set S' ∅ ) ∅
-  | bound_auth s _  => bound_frag (up s ∅) ∅
-  end.
-Inductive disjoint : Disjoint (bound sts) :=
-  | frag_frag_disjoint S1 S2 T1 T2 :
-     S1 ∩ S2 ≢ ∅ → T1 ∩ T2 ≡ ∅ → bound_frag S1 T1 ⊥ bound_frag S2 T2
-  | auth_frag_disjoint s S T1 T2 : s ∈ S → T1 ∩ T2 ≡ ∅ →
-                                   bound_auth s T1 ⊥ bound_frag S T2
-  | frag_auth_disjoint s S T1 T2 : s ∈ S → T1 ∩ T2 ≡ ∅ →
-                                   bound_frag S T1 ⊥ bound_auth s T2.
-Global Existing Instance disjoint.
-Global Instance op : Op (bound sts) := λ x1 x2,
-  match x1, x2 with
-  | bound_frag S1 T1, bound_frag S2 T2 => bound_frag (S1 ∩ S2) (T1 ∪ T2)
-  | bound_auth s T1, bound_frag _ T2 => bound_auth s (T1 ∪ T2)
-  | bound_frag _ T1, bound_auth s T2 => bound_auth s (T1 ∪ T2)
-  | bound_auth s T1, bound_auth _ T2 =>
-    bound_auth s (T1 ∪ T2)(* never happens *)
-  end.
-Global Instance minus : Minus (bound sts) := λ x1 x2,
-  match x1, x2 with
-  | bound_frag S1 T1, bound_frag S2 T2 => bound_frag
-                                            (up_set S1 (T1 ∖ T2)) (T1 ∖ T2)
-  | bound_auth s T1, bound_frag _ T2 => bound_auth s (T1 ∖ T2)
-  | bound_frag _ T2, bound_auth s T1 =>
-    bound_auth s (T1 ∖ T2) (* never happens *)
-  | bound_auth s T1, bound_auth _ T2 => bound_frag (up s (T1 ∖ T2)) (T1 ∖ T2)
-  end.
 
-Hint Extern 10 (base.equiv (A:=set _) _ _) => solve_elem_of : sts.
-Hint Extern 10 (¬(base.equiv (A:=set _) _ _)) => solve_elem_of : sts.
+(** Tactic setup *)
+Hint Resolve Step.
+Hint Extern 10 (equiv (A:=set _) _ _) => solve_elem_of : sts.
+Hint Extern 10 (¬equiv (A:=set _) _ _) => solve_elem_of : sts.
 Hint Extern 10 (_ ∈ _) => solve_elem_of : sts.
 Hint Extern 10 (_ ⊆ _) => solve_elem_of : sts.
-Instance: Equivalence ((≡) : relation (bound sts)).
-Proof.
-  split.
-  * by intros []; constructor.
-  * by destruct 1; constructor.
-  * destruct 1; inversion_clear 1; constructor; etransitivity; eauto.
-Qed.
-Instance framestep_proper : Proper ((≡) ==> (=) ==> (=) ==> impl) frame_step.
+
+(** ** Setoids *)
+Instance framestep_proper' : Proper ((≡) ==> (=) ==> (=) ==> impl) frame_step.
 Proof. intros ?? HT ?? <- ?? <-; destruct 1; econstructor; eauto with sts. Qed.
+Global Instance framestep_proper : Proper ((≡) ==> (=) ==> (=) ==> iff) frame_step.
+Proof. by intros ?? [??] ??????; split; apply framestep_proper'. Qed.
 Instance closed_proper' : Proper ((≡) ==> (≡) ==> impl) closed.
 Proof.
   intros ?? HT ?? HS; destruct 1;
     constructor; intros until 0; rewrite -?HS -?HT; eauto.
 Qed.
-Instance closed_proper : Proper ((≡) ==> (≡) ==> iff) closed.
+Global Instance closed_proper : Proper ((≡) ==> (≡) ==> iff) closed.
 Proof. by split; apply closed_proper'. Qed.
+Global Instance up_preserving : Proper ((=) ==> flip (⊆) ==> (⊆)) up.
+Proof.
+  intros s ? <- T T' HT ; apply elem_of_subseteq.
+  induction 1 as [|s1 s2 s3 [T1 T2]]; [constructor|].
+  eapply rtc_l; [eapply Frame_step with T1 T2|]; eauto with sts.
+Qed.
+Global Instance up_proper : Proper ((=) ==> (≡) ==> (≡)) up.
+Proof. by intros ??? ?? [??]; split; apply up_preserving. Qed.
+Global Instance up_set_preserving : Proper ((⊆) ==> flip (⊆) ==> (⊆)) up_set.
+Proof.
+  intros S1 S2 HS T1 T2 HT. rewrite /up_set.
+  f_equiv; last done. move =>s1 s2 Hs. simpl in HT. by apply up_preserving.
+Qed.
+Global Instance up_set_proper : Proper ((≡) ==> (≡) ==> (≡)) up_set.
+Proof. by intros S1 S2 [??] T1 T2 [??]; split; apply up_set_preserving. Qed.
+
+(** ** Properties of closure under frame steps *)
+Lemma closed_disjoint' S T s : closed S T → s ∈ S → tok s ∩ T ≡ ∅.
+Proof. intros [_ ? _]; solve_elem_of. Qed.
+Lemma closed_steps S T s1 s2 :
+  closed S T → s1 ∈ S → rtc (frame_step T) s1 s2 → s2 ∈ S.
+Proof. induction 3; eauto using closed_step. Qed.
 Lemma closed_op T1 T2 S1 S2 :
   closed S1 T1 → closed S2 T2 →
   T1 ∩ T2 ≡ ∅ → S1 ∩ S2 ≢ ∅ → closed (S1 ∩ S2) (T1 ∪ T2).
@@ -128,21 +93,16 @@ Proof.
   * apply Hstep1 with s3, Frame_step with T3 T4; auto with sts.
   * apply Hstep2 with s3, Frame_step with T3 T4; auto with sts.
 Qed.
-Instance up_preserving : Proper ((=) ==> flip (⊆) ==> (⊆)) up.
+Lemma step_closed s1 s2 T1 T2 S Tf :
+  step (s1,T1) (s2,T2) → closed S Tf → s1 ∈ S → T1 ∩ Tf ≡ ∅ →
+  s2 ∈ S ∧ T2 ∩ Tf ≡ ∅ ∧ tok s2 ∩ T2 ≡ ∅.
 Proof.
-  intros s ? <- T T' HT ; apply elem_of_subseteq.
-  induction 1 as [|s1 s2 s3 [T1 T2]]; [constructor|].
-  eapply rtc_l; [eapply Frame_step with T1 T2|]; eauto with sts.
+  inversion_clear 1 as [???? HR Hs1 Hs2]; intros [?? Hstep]??; split_ands; auto.
+  * eapply Hstep with s1, Frame_step with T1 T2; auto with sts.
+  * solve_elem_of -Hstep Hs1 Hs2.
 Qed.
-Instance up_proper : Proper ((=) ==> (≡) ==> (≡)) up.
-Proof. by intros ??? ?? [??]; split; apply up_preserving. Qed.
-Instance up_set_preserving : Proper ((⊆) ==> flip (⊆) ==> (⊆)) up_set.
-Proof.
-  intros S1 S2 HS T1 T2 HT. rewrite /up_set.
-  f_equiv; last done. move =>s1 s2 Hs. simpl in HT. by apply up_preserving.
-Qed.
-Instance up_set_proper : Proper ((≡) ==> (≡) ==> (≡)) up_set.
-Proof. by intros S1 S2 [??] T1 T2 [??]; split; apply up_set_preserving. Qed.
+
+(** ** Properties of the closure operators *)
 Lemma elem_of_up s T : s ∈ up s T.
 Proof. constructor. Qed.
 Lemma subseteq_up_set S T : S ⊆ up_set S T.
@@ -176,12 +136,82 @@ Proof.
   unfold up_set; rewrite elem_of_bind; intros (s'&Hstep&?).
   induction Hstep; eauto using closed_step.
 Qed.
-Global Instance dra : DRA (bound sts).
+End sts. End sts.
+
+Notation stsT := sts.stsT.
+Notation STS := sts.STS.
+
+(** * STSs form a disjoint RA *)
+(* This module should never be imported, uses the module [sts] below. *)
+Module sts_dra.
+Import sts.
+
+(* The type of bounds we can give to the state of an STS. This is the type
+   that we equip with an RA structure. *)
+Inductive car (sts : stsT) :=
+  | auth : state sts → set (token sts) → car sts
+  | frag : set (state sts) → set (token sts ) → car sts.
+Arguments auth {_} _ _.
+Arguments frag {_} _ _.
+
+Section sts_dra.
+Context {sts : stsT}.
+Infix "≼" := dra_included.
+Implicit Types S : states sts.
+Implicit Types T : tokens sts.
+
+Inductive sts_equiv : Equiv (car sts) :=
+  | auth_equiv s T1 T2 : T1 ≡ T2 → auth s T1 ≡ auth s T2
+  | frag_equiv S1 S2 T1 T2 : T1 ≡ T2 → S1 ≡ S2 → frag S1 T1 ≡ frag S2 T2.
+Existing Instance sts_equiv.
+Instance sts_valid : Valid (car sts) := λ x,
+  match x with auth s T => tok s ∩ T ≡ ∅ | frag S' T => closed S' T end.
+Instance sts_unit : Unit (car sts) := λ x,
+  match x with
+  | frag S' _ => frag (up_set S' ∅ ) ∅
+  | auth s _  => frag (up s ∅) ∅
+  end.
+Inductive sts_disjoint : Disjoint (car sts) :=
+  | frag_frag_disjoint S1 S2 T1 T2 :
+     S1 ∩ S2 ≢ ∅ → T1 ∩ T2 ≡ ∅ → frag S1 T1 ⊥ frag S2 T2
+  | auth_frag_disjoint s S T1 T2 :
+     s ∈ S → T1 ∩ T2 ≡ ∅ → auth s T1 ⊥ frag S T2
+  | frag_auth_disjoint s S T1 T2 :
+     s ∈ S → T1 ∩ T2 ≡ ∅ → frag S T1 ⊥ auth s T2.
+Existing Instance sts_disjoint.
+Instance sts_op : Op (car sts) := λ x1 x2,
+  match x1, x2 with
+  | frag S1 T1, frag S2 T2 => frag (S1 ∩ S2) (T1 ∪ T2)
+  | auth s T1, frag _ T2 => auth s (T1 ∪ T2)
+  | frag _ T1, auth s T2 => auth s (T1 ∪ T2)
+  | auth s T1, auth _ T2 => auth s (T1 ∪ T2)(* never happens *)
+  end.
+Instance sts_minus : Minus (car sts) := λ x1 x2,
+  match x1, x2 with
+  | frag S1 T1, frag S2 T2 => frag (up_set S1 (T1 ∖ T2)) (T1 ∖ T2)
+  | auth s T1, frag _ T2 => auth s (T1 ∖ T2)
+  | frag _ T2, auth s T1 => auth s (T1 ∖ T2) (* never happens *)
+  | auth s T1, auth _ T2 => frag (up s (T1 ∖ T2)) (T1 ∖ T2)
+  end.
+
+Hint Extern 10 (equiv (A:=set _) _ _) => solve_elem_of : sts.
+Hint Extern 10 (¬equiv (A:=set _) _ _) => solve_elem_of : sts.
+Hint Extern 10 (_ ∈ _) => solve_elem_of : sts.
+Hint Extern 10 (_ ⊆ _) => solve_elem_of : sts.
+Instance sts_equivalence: Equivalence ((≡) : relation (car sts)).
+Proof.
+  split.
+  * by intros []; constructor.
+  * by destruct 1; constructor.
+  * destruct 1; inversion_clear 1; constructor; etransitivity; eauto.
+Qed.
+Global Instance sts_dra : DRA (car sts).
 Proof.
   split.
   * apply _.
   * by do 2 destruct 1; constructor; setoid_subst.
   * by destruct 1; constructor; setoid_subst.
+  * by destruct 1; simpl; intros ?; setoid_subst.
   * by intros ? [|]; destruct 1; inversion_clear 1; constructor; setoid_subst.
   * by do 2 destruct 1; constructor; setoid_subst.
   * assert (∀ T T' S s,
@@ -233,50 +263,104 @@ Proof.
     unfold up_set; rewrite elem_of_bind; intros (?&s1&?&?&?).
     apply closed_steps with T2 s1; auto with sts.
 Qed.
-Lemma step_closed s1 s2 T1 T2 S Tf :
-  step (s1,T1) (s2,T2) → closed S Tf → s1 ∈ S → T1 ∩ Tf ≡ ∅ →
-  s2 ∈ S ∧ T2 ∩ Tf ≡ ∅ ∧ tok s2 ∩ T2 ≡ ∅.
-Proof.
-  inversion_clear 1 as [???? HR Hs1 Hs2]; intros [?? Hstep]??; split_ands; auto.
-  * eapply Hstep with s1, Frame_step with T1 T2; auto with sts.
-  * solve_elem_of -Hstep Hs1 Hs2.
-Qed.
-End sts_core.
+Canonical Structure RA : cmraT := validityRA (car sts).
+End sts_dra. End sts_dra.
+
+(** * The STS Resource Algebra *)
+(** Finally, the general theory of STS that should be used by users *)
+Notation stsRA := (@sts_dra.RA).
+
+Section sts_definitions.
+  Context {sts : stsT}.
+  Definition sts_auth (s : sts.state sts) (T : sts.tokens sts) : stsRA sts :=
+    to_validity (sts_dra.auth s T).
+  Definition sts_frag (S : sts.states sts) (T : sts.tokens sts) : stsRA sts :=
+    to_validity (sts_dra.frag S T).
+  Definition sts_frag_up (s : sts.state sts) (T : sts.tokens sts) : stsRA sts :=
+    sts_frag (sts.up s T) T.
+End sts_definitions.
+Instance: Params (@sts_auth) 2.
+Instance: Params (@sts_frag) 1.
+Instance: Params (@sts_frag_up) 2.
 
 Section stsRA.
-Context (sts : stsT).
+Import sts.
+Context {sts : stsT}.
+Implicit Types s : state sts.
+Implicit Types S : states sts.
+Implicit Types T : tokens sts.
 
-Canonical Structure RA := validityRA (bound sts).
-Definition auth (s : state sts) (T : set (token sts)) : RA :=
-  to_validity (bound_auth s T).
-Definition frag (S : set (state sts)) (T : set (token sts)) : RA :=
-  to_validity (bound_frag S T).
+(** Setoids *)
+Global Instance sts_auth_proper s : Proper ((≡) ==> (≡)) (sts_auth s).
+Proof. (* this proof is horrible *)
+  intros T1 T2 HT. rewrite /sts_auth.
+  by eapply to_validity_proper; try apply _; constructor.
+Qed.
+Global Instance sts_frag_proper : Proper ((≡) ==> (≡) ==> (≡)) (@sts_frag sts).
+Proof.
+  intros S1 S2 ? T1 T2 HT; rewrite /sts_auth.
+  by eapply to_validity_proper; try apply _; constructor.
+Qed.
+Global Instance sts_frag_up_proper s : Proper ((≡) ==> (≡)) (sts_frag_up s).
+Proof. intros T1 T2 HT. by rewrite /sts_frag_up HT. Qed.
 
-Lemma update_auth s1 s2 T1 T2 :
-  step sts (s1,T1) (s2,T2) → auth s1 T1 ~~> auth s2 T2.
+(** Validity *)
+Lemma sts_auth_valid s T : ✓ sts_auth s T ↔ tok s ∩ T ≡ ∅.
+Proof. split. by move=> /(_ 0). by intros ??. Qed.
+Lemma sts_frag_valid S T : ✓ sts_frag S T ↔ closed S T.
+Proof. split. by move=> /(_ 0). by intros ??. Qed.
+Lemma sts_frag_up_valid s T : tok s ∩ T ≡ ∅ → ✓ sts_frag_up s T.
+Proof. intros; by apply sts_frag_valid, closed_up. Qed.
+
+Lemma sts_auth_frag_valid_inv s S T1 T2 :
+  ✓ (sts_auth s T1 ⋅ sts_frag S T2) → s ∈ S.
+Proof. by move=> /(_ 0) [? [? Hdisj]]; inversion Hdisj. Qed.
+
+(** Op *)
+Lemma sts_op_auth_frag s S T :
+  s ∈ S → closed S T → sts_auth s ∅ ⋅ sts_frag S T ≡ sts_auth s T.
+Proof.
+  intros; split; [split|constructor; solve_elem_of]; simpl.
+  - intros (?&?&?); by apply closed_disjoint' with S.
+  - intros; split_ands. solve_elem_of+. done. constructor; solve_elem_of.
+Qed.
+Lemma sts_op_auth_frag_up s T :
+  tok s ∩ T ≡ ∅ → sts_auth s ∅ ⋅ sts_frag_up s T ≡ sts_auth s T.
+Proof. intros; apply sts_op_auth_frag; auto using elem_of_up, closed_up. Qed.
+
+(** Frame preserving updates *)
+Lemma sts_update_auth s1 s2 T1 T2 :
+  step (s1,T1) (s2,T2) → sts_auth s1 T1 ~~> sts_auth s2 T2.
 Proof.
   intros ?; apply validity_update; inversion 3 as [|? S ? Tf|]; subst.
-  destruct (step_closed sts s1 s2 T1 T2 S Tf) as (?&?&?); auto.
+  destruct (step_closed s1 s2 T1 T2 S Tf) as (?&?&?); auto.
   repeat (done || constructor).
 Qed.
 
-Lemma sts_update_frag S1 S2 (T : set (token sts)) :
-  S1 ⊆ S2 → closed sts S2 T →
-  frag S1 T ~~> frag S2 T.
+Lemma sts_update_frag S1 S2 T :
+  closed S2 T → S1 ⊆ S2 → sts_frag S1 T ~~> sts_frag S2 T.
 Proof.
-  move=>HS Hcl. eapply validity_update; inversion 3 as [|? S ? Tf|]; subst.
-  - split; first done. constructor; last done. solve_elem_of.
+  rewrite /sts_frag=> HS Hcl. apply validity_update.
+  inversion 3 as [|? S ? Tf|]; simplify_equality'.
+  - split; first done. constructor; [solve_elem_of|done].
   - split; first done. constructor; solve_elem_of.
 Qed.
 
-Lemma frag_included S1 S2 T1 T2 :
-  closed sts S2 T2 →
-  frag S1 T1 ≼ frag S2 T2 ↔ 
-  (closed sts S1 T1 ∧ ∃ Tf, T2 ≡ T1 ∪ Tf ∧ T1 ∩ Tf ≡ ∅ ∧
-                            S2 ≡ (S1 ∩ up_set sts S2 Tf)).
+Lemma sts_update_frag_up s1 S2 T :
+  closed S2 T → s1 ∈ S2 → sts_frag_up s1 T ~~> sts_frag S2 T.
 Proof.
+  intros; by apply sts_update_frag; [|intros ?; eauto using closed_steps].
+Qed.
+
+(** Inclusion *)
+Lemma sts_frag_included S1 S2 T1 T2 :
+  closed S2 T2 →
+  sts_frag S1 T1 ≼ sts_frag S2 T2 ↔
+  (closed S1 T1 ∧ ∃ Tf, T2 ≡ T1 ∪ Tf ∧ T1 ∩ Tf ≡ ∅ ∧ S2 ≡ S1 ∩ up_set S2 Tf).
+Proof. (* This should use some general properties of DRAs. To be improved
+when we have RAs back *)
   move=>Hcl2. split.
-  - intros [xf EQ]. destruct xf as [xf vf Hvf]. destruct xf as [Sf Tf|Sf Tf].
+  - intros [[[Sf Tf|Sf Tf] vf Hvf] EQ].
     { exfalso. inversion_clear EQ as [Hv EQ']. apply EQ' in Hcl2. simpl in Hcl2.
       inversion Hcl2. }
     inversion_clear EQ as [Hv EQ'].
@@ -286,31 +370,27 @@ Proof.
     inversion_clear Hdisj. split; last (exists Tf; split_ands); [done..|].
     apply (anti_symm (⊆)).
     + move=>s HS2. apply elem_of_intersection. split; first by apply HS.
-      by apply sts.subseteq_up_set.
+      by apply subseteq_up_set.
     + move=>s /elem_of_intersection [HS1 Hscl]. apply HS. split; first done.
       destruct Hscl as [s' [Hsup Hs']].
-      eapply sts.closed_steps; last (hnf in Hsup; eexact Hsup); first done.
+      eapply closed_steps; last (hnf in Hsup; eexact Hsup); first done.
       solve_elem_of +HS Hs'.
   - intros (Hcl1 & Tf & Htk & Hf & Hs).
-    exists (frag (up_set sts S2 Tf) Tf).
+    exists (sts_frag (up_set S2 Tf) Tf).
     split; first split; simpl;[|done|].
     + intros _. split_ands; first done.
-      * apply sts.closed_up_set; last by eapply sts.closed_ne.
-        move=>s Hs2. move:(closed_disjoint sts _ _ Hcl2 _ Hs2).
+      * apply closed_up_set; last by eapply closed_ne.
+        move=>s Hs2. move:(closed_disjoint _ _ Hcl2 _ Hs2).
         solve_elem_of +Htk.
-      * constructor; last done. rewrite -Hs. by eapply sts.closed_ne.
+      * constructor; last done. rewrite -Hs. by eapply closed_ne.
     + intros _. constructor; [ solve_elem_of +Htk | done].
 Qed.
 
-Lemma frag_included' S1 S2 T :
-  closed sts S2 T → closed sts S1 T →
-  S2 ≡ S1 ∩ sts.up_set sts S2 ∅ →
-  frag S1 T ≼ frag S2 T.
+Lemma sts_frag_included' S1 S2 T :
+  closed S2 T → closed S1 T → S2 ≡ S1 ∩ up_set S2 ∅ →
+  sts_frag S1 T ≼ sts_frag S2 T.
 Proof.
-  intros. apply frag_included; first done.
-  split; first done. exists ∅. split_ands; done || solve_elem_of+.
+  intros. apply sts_frag_included; split_ands; auto.
+  exists ∅; split_ands; done || solve_elem_of+.
 Qed.
-
 End stsRA.
-
-End sts.
