program_logic/sts.v
@@ -1,149 +1,134 @@
 From algebra Require Export sts.
-From algebra Require Import dra.
 From program_logic Require Export invariants ghost_ownership.
 Import uPred.
 
-Local Arguments valid _ _ !_ /.
-Local Arguments op _ _ !_ !_ /.
-Local Arguments unit _ _ !_ /.
-
-Module sts.
-(** This module is *not* meant to be imported. Instead, just use "sts.ctx" etc.
-    like you would use "auth_ctx" etc. *)
-Export algebra.sts.sts.
-
-Class InG Λ Σ (i : gid) (sts : stsT) := {
-  inG :> ghost_ownership.InG Λ Σ i (sts.RA sts);
-  inh :> Inhabited (state sts);
+Class STSInG Λ Σ (i : gid) (sts : stsT) := {
+  sts_inG :> ghost_ownership.InG Λ Σ i (stsRA sts);
+  sts_inhabited :> Inhabited (sts.state sts);
 }.
 
 Section definitions.
-  Context {Λ Σ} (i : gid) (sts : stsT) `{!InG Λ Σ i sts} (γ : gname).
-  Definition inv  (φ : state sts → iPropG Λ Σ) : iPropG Λ Σ :=
-    (∃ s, own i γ (auth sts s ∅) ★ φ s)%I.
-  Definition in_states (S : set (state sts)) (T: set (token sts)) : iPropG Λ Σ:=
-    own i γ (frag sts S T)%I.
-  Definition in_state (s : state sts) (T: set (token sts)) : iPropG Λ Σ :=
-    in_states (up sts s T) T.
-  Definition ctx (N : namespace) (φ : state sts → iPropG Λ Σ) : iPropG Λ Σ :=
-    invariants.inv N (inv φ).
+  Context {Λ Σ} (i : gid) (sts : stsT) `{!STSInG Λ Σ i sts} (γ : gname).
+  Import sts.
+  Definition sts_inv (φ : state sts → iPropG Λ Σ) : iPropG Λ Σ :=
+    (∃ s, own i γ (sts_auth s ∅) ★ φ s)%I.
+  Definition sts_ownS (S : states sts) (T : tokens sts) : iPropG Λ Σ:=
+    own i γ (sts_frag S T).
+  Definition sts_own (s : state sts) (T : tokens sts) : iPropG Λ Σ :=
+    own i γ (sts_frag_up s T).
+  Definition sts_ctx (N : namespace) (φ: state sts → iPropG Λ Σ) : iPropG Λ Σ :=
+    inv N (sts_inv φ).
 End definitions.
-Instance: Params (@inv) 6.
-Instance: Params (@in_states) 6.
-Instance: Params (@in_state) 6.
-Instance: Params (@ctx) 7.
+Instance: Params (@sts_inv) 6.
+Instance: Params (@sts_ownS) 6.
+Instance: Params (@sts_own) 7.
+Instance: Params (@sts_ctx) 7.
 
 Section sts.
-  Context {Λ Σ} (i : gid) (sts : stsT) `{!InG Λ Σ StsI sts}.
-  Context (φ : state sts → iPropG Λ Σ).
+  Context {Λ Σ} (i : gid) (sts : stsT) `{!STSInG Λ Σ StsI sts}.
+  Context (φ : sts.state sts → iPropG Λ Σ).
   Implicit Types N : namespace.
   Implicit Types P Q R : iPropG Λ Σ.
   Implicit Types γ : gname.
+  Implicit Types S : sts.states sts.
+  Implicit Types T : sts.tokens sts.
+
+  (** Setoids *)
+  Global Instance sts_inv_ne n γ :
+    Proper (pointwise_relation _ (dist n) ==> dist n) (sts_inv StsI sts γ).
+  Proof. by intros φ1 φ2 Hφ; rewrite /sts_inv; setoid_rewrite Hφ. Qed.
+  Global Instance sts_inv_proper γ :
+    Proper (pointwise_relation _ (≡) ==> (≡)) (sts_inv StsI sts γ).
+  Proof. by intros φ1 φ2 Hφ; rewrite /sts_inv; setoid_rewrite Hφ. Qed.
+  Global Instance sts_ownS_proper γ :
+    Proper ((≡) ==> (≡) ==> (≡)) (sts_ownS StsI sts γ).
+  Proof. intros S1 S2 HS T1 T2 HT. by rewrite /sts_ownS HS HT. Qed.
+  Global Instance sts_own_proper γ s :
+    Proper ((≡) ==> (≡)) (sts_ownS StsI sts γ s).
+  Proof. intros T1 T2 HT. by rewrite /sts_ownS HT. Qed.
+  Global Instance sts_ctx_ne n γ N :
+    Proper (pointwise_relation _ (dist n) ==> dist n) (sts_ctx StsI sts γ N).
+  Proof. by intros φ1 φ2 Hφ; rewrite /sts_ctx Hφ. Qed.
+  Global Instance sts_ctx_proper γ N :
+    Proper (pointwise_relation _ (≡) ==> (≡)) (sts_ctx StsI sts γ N).
+  Proof. by intros φ1 φ2 Hφ; rewrite /sts_ctx Hφ. Qed.
 
   (* The same rule as implication does *not* hold, as could be shown using
      sts_frag_included. *)
-  Lemma in_states_weaken E γ S1 S2 T :
-    S1 ⊆ S2 → closed sts S2 T →
-    in_states StsI sts γ S1 T ⊑ pvs E E (in_states StsI sts γ S2 T).
-  Proof.
-    rewrite /in_states=>Hs Hcl. apply own_update, sts_update_frag; done.
-  Qed.
+  Lemma sts_ownS_weaken E γ S1 S2 T :
+    S1 ⊆ S2 → sts.closed S2 T →
+    sts_ownS StsI sts γ S1 T ⊑ pvs E E (sts_ownS StsI sts γ S2 T).
+  Proof. intros. by apply own_update, sts_update_frag. Qed.
 
-  Lemma in_state_states E γ s S T :
-    s ∈ S → closed sts S T →
-    in_state StsI sts γ s T ⊑ pvs E E (in_states StsI sts γ S T).
-  Proof.
-    move=>Hs Hcl. apply in_states_weaken; last done.
-    move=>s' Hup. eapply closed_steps in Hcl;last (hnf in Hup; eexact Hup);done.
-  Qed.
+  Lemma sts_own_weaken E γ s S T :
+    s ∈ S → sts.closed S T →
+    sts_own StsI sts γ s T ⊑ pvs E E (sts_ownS StsI sts γ S T).
+  Proof. intros. by apply own_update, sts_update_frag_up. Qed.
 
-  Lemma alloc N s :
-    φ s ⊑ pvs N N (∃ γ, ctx StsI sts γ N φ ∧
-                        in_state StsI sts γ s (set_all ∖ sts.(tok) s)).
+  Lemma sts_alloc N s :
+    φ s ⊑ pvs N N (∃ γ, sts_ctx StsI sts γ N φ ∧
+                        sts_own StsI sts γ s (set_all ∖ sts.tok s)).
   Proof.
     eapply sep_elim_True_r.
-    { eapply (own_alloc StsI (auth sts s (set_all ∖ sts.(tok) s)) N).
-      apply discrete_valid=>/=. solve_elem_of. }
+    { apply (own_alloc StsI (sts_auth s (set_all ∖ sts.tok s)) N).
+      apply sts_auth_valid; solve_elem_of. }
     rewrite pvs_frame_l. apply pvs_strip_pvs.
     rewrite sep_exist_l. apply exist_elim=>γ. rewrite -(exist_intro γ).
-    transitivity (▷ inv StsI sts γ φ ★
-                    in_state StsI sts γ s (set_all ∖ sts.(tok) s))%I.
-    { rewrite /inv -later_intro -(exist_intro s).
-      rewrite [(_ ★ φ _)%I]comm -assoc. apply sep_mono; first done.
-      rewrite -own_op. apply equiv_spec, own_proper.
-      split; first split; simpl.
-      - intros; solve_elem_of+.
-      - intros _. split_ands; first by solve_elem_of+.
-        + apply closed_up. solve_elem_of+.
-        + constructor; last solve_elem_of+. apply sts.elem_of_up. 
-      - intros _. constructor. solve_elem_of+. }
-    rewrite (inv_alloc N) /ctx pvs_frame_r. apply pvs_mono.
+    transitivity (▷ sts_inv StsI sts γ φ ★
+                    sts_own StsI sts γ s (set_all ∖ sts.tok s))%I.
+    { rewrite /sts_inv -later_intro -(exist_intro s).
+      rewrite [(_ ★ φ _)%I]comm -assoc. apply sep_mono_r.
+      by rewrite -own_op sts_op_auth_frag_up; last solve_elem_of+. }
+    rewrite (inv_alloc N) /sts_ctx pvs_frame_r.
     by rewrite always_and_sep_l.
   Qed.
 
-  Lemma opened E γ S T :
-    (▷ inv StsI sts γ φ ★ in_states StsI sts γ S T)
-      ⊑ pvs E E (∃ s, ■ (s ∈ S) ★ ▷ φ s ★ own StsI γ (auth sts s T)).
+  Lemma sts_opened E γ S T :
+    (▷ sts_inv StsI sts γ φ ★ sts_ownS StsI sts γ S T)
+    ⊑ pvs E E (∃ s, ■ (s ∈ S) ★ ▷ φ s ★ own StsI γ (sts_auth s T)).
   Proof.
-    rewrite /inv /in_states later_exist sep_exist_r. apply exist_elim=>s.
+    rewrite /sts_inv /sts_ownS later_exist sep_exist_r. apply exist_elim=>s.
     rewrite later_sep pvs_timeless !pvs_frame_r. apply pvs_mono.
     rewrite -(exist_intro s).
     rewrite [(_ ★ ▷φ _)%I]comm -!assoc -own_op -[(▷φ _ ★ _)%I]comm.
     rewrite own_valid_l discrete_validI.
-    rewrite -!assoc. apply const_elim_sep_l=>-[_ [Hcl Hdisj]].
-    simpl in Hdisj, Hcl. inversion_clear Hdisj. rewrite const_equiv // left_id.
-    rewrite comm. apply sep_mono; first done.
-    apply equiv_spec, own_proper. split; first split; simpl.
-    - intros Hdisj. split_ands; first by solve_elem_of+.
-      + done.
-      + constructor; [done | solve_elem_of-].
-    - intros _. by eapply closed_disjoint'.
-    - intros _. constructor. solve_elem_of+.
+    rewrite -!assoc. apply const_elim_sep_l=> Hvalid.
+    assert (s ∈ S) by (by eapply sts_auth_frag_valid_inv, discrete_valid).
+    rewrite const_equiv // left_id comm sts_op_auth_frag //.
+    (* this is horrible, but will be fixed whenever we have RAs back *)
+    by rewrite -sts_frag_valid; eapply cmra_valid_op_r, discrete_valid.
   Qed.
 
-  Lemma closing E γ s T s' T' :
-    step sts (s, T) (s', T') →
-    (▷ φ s' ★ own StsI γ (auth sts s T))
-    ⊑ pvs E E (▷ inv StsI sts γ φ ★ in_state StsI sts γ s' T').
+  Lemma sts_closing E γ s T s' T' :
+    sts.step (s, T) (s', T') →
+    (▷ φ s' ★ own StsI γ (sts_auth s T))
+    ⊑ pvs E E (▷ sts_inv StsI sts γ φ ★ sts_own StsI sts γ s' T').
   Proof.
-    intros Hstep. rewrite /inv /in_states -(exist_intro s').
+    intros Hstep. rewrite /sts_inv /sts_own -(exist_intro s').
     rewrite later_sep [(_ ★ ▷φ _)%I]comm -assoc.
-    rewrite -pvs_frame_l. apply sep_mono; first done.
-    rewrite -later_intro.
+    rewrite -pvs_frame_l. apply sep_mono_r. rewrite -later_intro.
     rewrite own_valid_l discrete_validI. apply const_elim_sep_l=>Hval.
-    simpl in Hval. transitivity (pvs E E (own StsI γ (auth sts s' T'))).
-    { by apply own_update, sts.update_auth. }
-    apply pvs_mono. rewrite -own_op. apply equiv_spec, own_proper.
-    split; first split; simpl.
-    - intros _.
-      set Tf := set_all ∖ sts.(tok) s ∖ T.
-      assert (closed sts (up sts s Tf) Tf).
-      { apply closed_up. rewrite /Tf. solve_elem_of+. }
-      eapply step_closed; [done..| |].
-      + apply elem_of_up.
-      + rewrite /Tf. solve_elem_of+.
-    - intros ?. split_ands; first by solve_elem_of+.
-      + apply closed_up. done.
-      + constructor; last solve_elem_of+. apply elem_of_up.
-    - intros _. constructor. solve_elem_of+.
+    transitivity (pvs E E (own StsI γ (sts_auth s' T'))).
+    { by apply own_update, sts_update_auth. }
+    by rewrite -own_op sts_op_auth_frag_up; last by inversion_clear Hstep.
   Qed.
 
   Context {V} (fsa : FSA Λ (globalF Σ) V) `{!FrameShiftAssertion fsaV fsa}.
 
-  Lemma states_fsa E N P (Q : V → iPropG Λ Σ) γ S T :
+  Lemma sts_fsaS E N P (Q : V → iPropG Λ Σ) γ S T :
     fsaV → nclose N ⊆ E →
-    P ⊑ ctx StsI sts γ N φ →
-    P ⊑ (in_states StsI sts γ S T ★ ∀ s,
+    P ⊑ sts_ctx StsI sts γ N φ →
+    P ⊑ (sts_ownS StsI sts γ S T ★ ∀ s,
           ■ (s ∈ S) ★ ▷ φ s -★
           fsa (E ∖ nclose N) (λ x, ∃ s' T',
-            ■ (step sts (s, T) (s', T')) ★ ▷ φ s' ★
-            (in_state StsI sts γ s' T' -★ Q x))) →
+            ■ sts.step (s, T) (s', T') ★ ▷ φ s' ★
+            (sts_own StsI sts γ s' T' -★ Q x))) →
     P ⊑ fsa E Q.
   Proof.
-    rewrite /ctx=>? HN Hinv Hinner.
+    rewrite /sts_ctx=>? HN Hinv Hinner.
     eapply (inv_fsa fsa); eauto. rewrite Hinner=>{Hinner Hinv P HN}.
     apply wand_intro_l. rewrite assoc.
-    rewrite (opened (E ∖ N)) !pvs_frame_r !sep_exist_r.
+    rewrite (sts_opened (E ∖ N)) !pvs_frame_r !sep_exist_r.
     apply (fsa_strip_pvs fsa). apply exist_elim=>s.
     rewrite (forall_elim s). rewrite [(▷_ ★ _)%I]comm.
     (* Getting this wand eliminated is really annoying. *)
@@ -154,24 +139,19 @@ Section sts.
     rewrite sep_exist_l; apply exist_elim=>T'.
     rewrite comm -!assoc. apply const_elim_sep_l=>-Hstep.
     rewrite assoc [(_ ★ (_ -★ _))%I]comm -assoc.
-    rewrite (closing (E ∖ N)) //; [].
+    rewrite (sts_closing (E ∖ N)) //; [].
     rewrite pvs_frame_l. apply pvs_mono.
     by rewrite assoc [(_ ★ ▷_)%I]comm -assoc wand_elim_l.
   Qed.
 
-  Lemma state_fsa E N P (Q : V → iPropG Λ Σ) γ s0 T :
+  Lemma sts_fsa E N P (Q : V → iPropG Λ Σ) γ s0 T :
     fsaV → nclose N ⊆ E →
-    P ⊑ ctx StsI sts γ N φ →
-    P ⊑ (in_state StsI sts γ s0 T ★ ∀ s,
-          ■ (s ∈ up sts s0 T) ★ ▷ φ s -★
+    P ⊑ sts_ctx StsI sts γ N φ →
+    P ⊑ (sts_own StsI sts γ s0 T ★ ∀ s,
+          ■ (s ∈ sts.up s0 T) ★ ▷ φ s -★
           fsa (E ∖ nclose N) (λ x, ∃ s' T',
-            ■ (step sts (s, T) (s', T')) ★ ▷ φ s' ★
-            (in_state StsI sts γ s' T' -★ Q x))) →
+            ■ (sts.step (s, T) (s', T')) ★ ▷ φ s' ★
+            (sts_own StsI sts γ s' T' -★ Q x))) →
     P ⊑ fsa E Q.
-  Proof.
-    rewrite {1}/state. apply states_fsa.
-  Qed.
-
-End sts.
-
+  Proof. apply sts_fsaS. Qed.
 End sts.
